tuned

src/HOL/IMP/Abs_Int0_const.thy
@@ -85,21 +85,18 @@ qed
 
 text{* Termination: *}
 
+definition "m_const x = (case x of Const _ \<Rightarrow> 1 | Any \<Rightarrow> 0)"
+
 lemma measure_const:
-  "(strict{(x::const,y). x \<sqsubseteq> y})^-1 \<subseteq>
-  measure(%x. case x of Const _ \<Rightarrow> 1 | Any \<Rightarrow> 0)"
-by(auto split: const.splits)
+  "(strict{(x::const,y). x \<sqsubseteq> y})^-1 \<subseteq> measure m_const"
+by(auto simp: m_const_def split: const.splits)
 
 lemma measure_const_eq:
-  "\<forall> x y::const. x \<sqsubseteq> y \<and> y \<sqsubseteq> x \<longrightarrow> (%x. case x of Const _ \<Rightarrow> 1 | Any \<Rightarrow> 0) x = (%x. case x of Const _ \<Rightarrow> 1 | Any \<Rightarrow> 0) y"
-by(auto split: const.splits)
-
-lemma acc_const_st: "Abs_Int0.acc{(x::const st,y). x \<sqsubseteq> y}"
-by(rule wf_subset[OF wf_measure measure_st[OF measure_const measure_const_eq]])
+  "\<forall> x y::const. x \<sqsubseteq> y \<and> y \<sqsubseteq> x \<longrightarrow> m_const x = m_const y"
+by(auto simp: m_const_def split: const.splits)
 
 lemma "EX c'. AI_const c = Some c'"
-by(metis AI_def lpfpc_termination[OF acc_const_st, where f = "step_const \<top>",
-  OF mono_step'[OF le_refl] strip_step'])
+by(rule AI_Some_measure[OF measure_const measure_const_eq])
 
 
 subsubsection "Tests"
